src/coq/Theory/InterpreterMCFG.v
@@ -25,34 +25,34 @@ Section InterpreterMCFG.
    This gives us a _vertical_ notion of compositionality.
    *)
 
-  Definition interp_to_L1 {R} user_intrinsics (t: itree L0 R) g :=
-    let uvalue_trace       := interp_intrinsics user_intrinsics t in
+  Definition interp_to_L1 {R} (t: itree L0 R) g :=
+    let uvalue_trace       := interp_intrinsics t in
     let L1_trace           := interp_global uvalue_trace g in
     L1_trace.
 
-  Definition interp_to_L2 {R} user_intrinsics (t: itree L0 R) g l :=
-    let uvalue_trace   := interp_intrinsics user_intrinsics t in
+  Definition interp_to_L2 {R} (t: itree L0 R) g l :=
+    let uvalue_trace   := interp_intrinsics t in
     let L1_trace       := interp_global uvalue_trace g in
     let L2_trace       := interp_local_stack (handle_local (v:=uvalue)) L1_trace l in
     L2_trace.
 
-  Definition interp_to_L3 {R} user_intrinsics (t: itree L0 R) g l m :=
-    let uvalue_trace   := interp_intrinsics user_intrinsics t in
+  Definition interp_to_L3 {R} (t: itree L0 R) g l m :=
+    let uvalue_trace   := interp_intrinsics t in
     let L1_trace       := interp_global uvalue_trace g in
     let L2_trace       := interp_local_stack (handle_local (v:=uvalue)) L1_trace l in
     let L3_trace       := interp_memory L2_trace m in
     L3_trace.
 
-  Definition interp_to_L4 {R} RR user_intrinsics (t: itree L0 R) g l m :=
-    let uvalue_trace   := interp_intrinsics user_intrinsics t in
+  Definition interp_to_L4 {R} RR (t: itree L0 R) g l m :=
+    let uvalue_trace   := interp_intrinsics t in
     let L1_trace       := interp_global uvalue_trace g in
     let L2_trace       := interp_local_stack (handle_local (v:=uvalue)) L1_trace l in
     let L3_trace       := interp_memory L2_trace m in
     let L4_trace       := model_undef RR L3_trace in
     L4_trace.
 
-  Definition interp_to_L5 {R} RR user_intrinsics (t: itree L0 R) g l m :=
-    let uvalue_trace   := interp_intrinsics user_intrinsics t in
+  Definition interp_to_L5 {R} RR (t: itree L0 R) g l m :=
+    let uvalue_trace   := interp_intrinsics t in
     let L1_trace       := interp_global uvalue_trace g in
     let L2_trace       := interp_local_stack (handle_local (v:=uvalue)) L1_trace l in
     let L3_trace       := interp_memory L2_trace m in
@@ -60,16 +60,16 @@ Section InterpreterMCFG.
     model_UB RR L4_trace.
 
   (* The interpreter stray away from the model starting from the fourth layer: we pick an arbitrary valid path of execution *)
-  Definition interp_to_L4_exec {R} user_intrinsics (t: itree L0 R) g l m :=
-    let uvalue_trace   := interp_intrinsics user_intrinsics t in
+  Definition interp_to_L4_exec {R} (t: itree L0 R) g l m :=
+    let uvalue_trace   := interp_intrinsics t in
     let L1_trace       := interp_global uvalue_trace g in
     let L2_trace       := interp_local_stack (handle_local (v:=uvalue)) L1_trace l in
     let L3_trace       := interp_memory L2_trace m in
     let L4_trace       := exec_undef L3_trace in
     L4_trace.
 
-  Definition interp_to_L5_exec {R} user_intrinsics (t: itree L0 R) g l m :=
-    let uvalue_trace   := interp_intrinsics user_intrinsics t in
+  Definition interp_to_L5_exec {R} (t: itree L0 R) g l m :=
+    let uvalue_trace   := interp_intrinsics t in
     let L1_trace       := interp_global uvalue_trace g in
     let L2_trace       := interp_local_stack (handle_local (v:=uvalue)) L1_trace l in
     let L3_trace       := interp_memory L2_trace m in
@@ -79,9 +79,9 @@ Section InterpreterMCFG.
   Section Structural_Lemmas.
 
     Lemma interp_to_L1_bind :
-      forall ui {R S} (t: itree L0 R) (k: R -> itree L0 S) g, 
-        interp_to_L1 ui (ITree.bind t k) g ≈
-                     (ITree.bind (interp_to_L1 ui t g) (fun '(g',x) => interp_to_L1 ui (k x) g')).
+      forall {R S} (t: itree L0 R) (k: R -> itree L0 S) g, 
+        interp_to_L1 (ITree.bind t k) g ≈
+                     (ITree.bind (interp_to_L1 t g) (fun '(g',x) => interp_to_L1 (k x) g')).
     Proof.
       intros.
       unfold interp_to_L1.
@@ -89,16 +89,16 @@ Section InterpreterMCFG.
       apply eutt_eq_bind; intros (? & ?); reflexivity.
     Qed.
 
-    Lemma interp_to_L1_ret : forall ui (R : Type) g (x : R), interp_to_L1 ui (Ret x) g ≈ Ret (g,x).
+    Lemma interp_to_L1_ret : forall (R : Type) g (x : R), interp_to_L1 (Ret x) g ≈ Ret (g,x).
     Proof.
       intros; unfold interp_to_L1.
       rewrite interp_intrinsics_ret, interp_global_ret; reflexivity.
     Qed.
 
     Lemma interp_to_L2_bind :
-      forall ui {R S} (t: itree L0 R) (k: R -> itree L0 S) g l,
-        interp_to_L2 ui (ITree.bind t k) g l ≈
-                     (ITree.bind (interp_to_L2 ui t g l) (fun '(g',(l',x)) => interp_to_L2 ui (k x) l' g')).
+      forall {R S} (t: itree L0 R) (k: R -> itree L0 S) g l,
+        interp_to_L2 (ITree.bind t k) g l ≈
+                     (ITree.bind (interp_to_L2 t g l) (fun '(g',(l',x)) => interp_to_L2 (k x) l' g')).
     Proof.
       intros.
       unfold interp_to_L2.
@@ -106,16 +106,16 @@ Section InterpreterMCFG.
       apply eutt_eq_bind; intros (? & ? & ?); reflexivity.
     Qed.
 
-    Lemma interp_to_L2_ret : forall ui (R : Type) g l (x : R), interp_to_L2 ui (Ret x) g l ≈ Ret (l, (g, x)).
+    Lemma interp_to_L2_ret : forall (R : Type) g l (x : R), interp_to_L2 (Ret x) g l ≈ Ret (l, (g, x)).
     Proof.
       intros; unfold interp_to_L2.
       rewrite interp_intrinsics_ret, interp_global_ret, interp_local_stack_ret; reflexivity.
     Qed.
 
     Lemma interp_to_L3_bind :
-      forall ui {R S} (t: itree L0 R) (k: R -> itree L0 S) g l m,
-        interp_to_L3 ui (ITree.bind t k) g l m ≈
-                     (ITree.bind (interp_to_L3 ui t g l m) (fun '(m',(l',(g',x))) => interp_to_L3 ui (k x) g' l' m')).
+      forall {R S} (t: itree L0 R) (k: R -> itree L0 S) g l m,
+        interp_to_L3 (ITree.bind t k) g l m ≈
+                     (ITree.bind (interp_to_L3 t g l m) (fun '(m',(l',(g',x))) => interp_to_L3 (k x) g' l' m')).
     Proof.
       intros.
       unfold interp_to_L3.
@@ -123,14 +123,14 @@ Section InterpreterMCFG.
       apply eutt_eq_bind; intros (? & ? & ? & ?); reflexivity.
     Qed.
 
-    Lemma interp_to_L3_ret : forall ui (R : Type) g l m (x : R), interp_to_L3 ui (Ret x) g l m ≈ Ret (m, (l, (g,x))).
+    Lemma interp_to_L3_ret : forall (R : Type) g l m (x : R), interp_to_L3 (Ret x) g l m ≈ Ret (m, (l, (g,x))).
     Proof.
       intros; unfold interp_to_L3.
       rewrite interp_intrinsics_ret, interp_global_ret, interp_local_stack_ret, interp_memory_ret; reflexivity.
     Qed.
 
-    Global Instance eutt_interp_to_L1 (defs: intrinsic_definitions) {T}:
-      Proper (eutt Logic.eq ==> Logic.eq ==> eutt Logic.eq) (@interp_to_L1 T defs).
+    Global Instance eutt_interp_to_L1 {T}:
+      Proper (eutt Logic.eq ==> Logic.eq ==> eutt Logic.eq) (@interp_to_L1 T).
     Proof.
       repeat intro.
       unfold interp_to_L1.
@@ -138,8 +138,8 @@ Section InterpreterMCFG.
       reflexivity.
     Qed.
 
-    Global Instance eutt_interp_to_L2 (defs: intrinsic_definitions) {T}:
-      Proper (eutt Logic.eq ==> Logic.eq ==> Logic.eq ==> eutt Logic.eq) (@interp_to_L2 T defs).
+    Global Instance eutt_interp_to_L2 {T}:
+      Proper (eutt Logic.eq ==> Logic.eq ==> Logic.eq ==> eutt Logic.eq) (@interp_to_L2 T).
     Proof.
       repeat intro.
       unfold interp_to_L2.
@@ -147,8 +147,8 @@ Section InterpreterMCFG.
       reflexivity.
     Qed.
 
-    Global Instance eutt_interp_to_L3 (defs: intrinsic_definitions) {T}:
-      Proper (eutt Logic.eq ==> Logic.eq ==> Logic.eq ==> Logic.eq ==> eutt Logic.eq) (@interp_to_L3 T defs).
+    Global Instance eutt_interp_to_L3 {T}:
+      Proper (eutt Logic.eq ==> Logic.eq ==> Logic.eq ==> Logic.eq ==> eutt Logic.eq) (@interp_to_L3 T).
     Proof.
       repeat intro.
       unfold interp_to_L3.
@@ -157,11 +157,11 @@ Section InterpreterMCFG.
     Qed.
 
     (* NOTEYZ: This can probably be refined to [eqit eq] instead of [eutt eq], but I don't think it matters to us *)
-    Lemma interp_to_L3_vis (defs: IS.intrinsic_definitions):
+    Lemma interp_to_L3_vis: 
       forall T R (e : L0 T) (k : T -> itree L0 R) g l m,
-        interp_to_L3 defs (Vis e k) g l m ≈ 
-                     ITree.bind (interp_to_L3 defs (trigger e) g l m)
-                     (fun '(m, (l, (g, x)))=> interp_to_L3 defs (k x) g l m).
+        interp_to_L3 (Vis e k) g l m ≈ 
+                     ITree.bind (interp_to_L3 (trigger e) g l m)
+                     (fun '(m, (l, (g, x)))=> interp_to_L3 (k x) g l m).
     Proof.
       intros.
       unfold interp_to_L3.
@@ -172,18 +172,15 @@ Section InterpreterMCFG.
       rewrite Eq.bind_bind.
       apply eutt_eq_bind.
       intros (? & ? & ? & ?).
-      do 2 match goal with
-             |- context[interp ?x ?t] => replace (interp x t) with (interp_intrinsics defs t) by reflexivity
-           end. 
       rewrite interp_intrinsics_ret, interp_global_ret, interp_local_stack_ret, interp_memory_ret, bind_ret_l.
       reflexivity.
     Qed.
 
-    Lemma interp_to_L3_bind_trigger (defs: IS.intrinsic_definitions):
+    Lemma interp_to_L3_bind_trigger :
       forall T R (e : L0 T) (k : T -> itree L0 R) g l m,
-        interp_to_L3 defs (ITree.bind (trigger e) k) g l m ≈ 
-                     ITree.bind (interp_to_L3 defs (trigger e) g l m)
-                     (fun '(m, (l, (g, x)))=> interp_to_L3 defs (k x) g l m).
+        interp_to_L3 (ITree.bind (trigger e) k) g l m ≈ 
+                     ITree.bind (interp_to_L3 (trigger e) g l m)
+                     (fun '(m, (l, (g, x)))=> interp_to_L3 (k x) g l m).
     Proof.
       intros.
       rewrite bind_trigger.
@@ -191,8 +188,8 @@ Section InterpreterMCFG.
       reflexivity.
     Qed.
 
-    Lemma interp_to_L3_GW : forall defs id g l m v,
-        interp_to_L3 defs (trigger (GlobalWrite id v)) g l m ≈ ret (m,(l,(Maps.add id v g,tt))).
+    Lemma interp_to_L3_GW : forall id g l m v,
+        interp_to_L3 (trigger (GlobalWrite id v)) g l m ≈ ret (m,(l,(Maps.add id v g,tt))).
     Proof.
       intros.
       unfold interp_to_L3.
@@ -204,10 +201,10 @@ Section InterpreterMCFG.
       reflexivity.
     Qed.
 
-    Lemma interp_cfg_to_L3_LM : forall defs t a size offset g l m v bytes concrete_id,
+    Lemma interp_cfg_to_L3_LM : forall t a size offset g l m v bytes concrete_id,
         get_logical_block m a = Some (LBlock size bytes concrete_id) ->
         deserialize_sbytes (lookup_all_index offset (sizeof_dtyp t) bytes SUndef) t = v ->
-        interp_to_L3 defs (trigger (Load t (DVALUE_Addr (a, offset)))) g l m ≈ Ret (m,(l,(g,v))).
+        interp_to_L3 (trigger (Load t (DVALUE_Addr (a, offset)))) g l m ≈ Ret (m,(l,(g,v))).
     Proof.
       intros * LUL EQ.
       unfold interp_to_L3.
@@ -235,11 +232,11 @@ Section InterpreterMCFG.
     Qed.
 
     Lemma interp_to_L3_alloca :
-      forall (defs : intrinsic_definitions) (m : memory_stack) (t : dtyp) (g : global_env) l,
+      forall (m : memory_stack) (t : dtyp) (g : global_env) l,
         non_void t ->
         exists m' a',
           allocate m t = inr (m', a') /\
-          interp_to_L3 defs (trigger (Alloca t)) g l m ≈ ret (m', (l, (g, DVALUE_Addr a'))).
+          interp_to_L3 (trigger (Alloca t)) g l m ≈ ret (m', (l, (g, DVALUE_Addr a'))).
     Proof.
       intros * NV.
       unfold interp_to_L3.
@@ -275,17 +272,17 @@ End InterpreterMCFG.
 
 Ltac fold_L1 :=
   match goal with
-    |- context[interp_global (interp_intrinsics ?ui ?p) ?g] =>
-    replace (interp_global (interp_intrinsics ui p) g) with
-    (interp_to_L1 ui p g) by reflexivity
+    |- context[interp_global (interp_intrinsics ?p) ?g] =>
+    replace (interp_global (interp_intrinsics p) g) with
+    (interp_to_L1 p g) by reflexivity
   end.
 
 Ltac fold_L2 :=
   match goal with
     |- context[interp_local_stack ?h
-                                 (interp_global (interp_intrinsics ?ui ?p) ?g) ?l] =>
-    replace (interp_local_stack h (interp_global (interp_intrinsics ui p) g) l) with
-    (interp_to_L2 ui p g l) by reflexivity
+                                 (interp_global (interp_intrinsics ?p) ?g) ?l] =>
+    replace (interp_local_stack h (interp_global (interp_intrinsics p) g) l) with
+    (interp_to_L2 p g l) by reflexivity
   end.
 
 Ltac fold_L3 :=
@@ -293,9 +290,9 @@ Ltac fold_L3 :=
     |- context[
           interp_memory
             (interp_local_stack ?h
-                                (interp_global (interp_intrinsics ?ui ?p) ?g) ?l) ?m] =>
-    replace (interp_memory (interp_local_stack h (interp_global (interp_intrinsics ui p) g) l) m) with
-    (interp_to_L3 ui p g l m) by reflexivity
+                                (interp_global (interp_intrinsics ?p) ?g) ?l) ?m] =>
+    replace (interp_memory (interp_local_stack h (interp_global (interp_intrinsics p) g) l) m) with
+    (interp_to_L3 p g l m) by reflexivity
   end.
 
 Ltac fold_L4 :=
@@ -304,14 +301,14 @@ Ltac fold_L4 :=
           model_undef ?RR
             (interp_memory
                (interp_local_stack ?h
-                                   (interp_global (interp_intrinsics ?ui ?p) ?g) ?l) ?m)] =>
-    replace (model_undef ?RR (interp_memory (interp_local_stack h (interp_global (interp_intrinsics ui p) g) l) m)) with
-    (interp_to_L4 RR ui p g l m) by reflexivity
+                                   (interp_global (interp_intrinsics ?p) ?g) ?l) ?m)] =>
+    replace (model_undef ?RR (interp_memory (interp_local_stack h (interp_global (interp_intrinsics p) g) l) m)) with
+    (interp_to_L4 RR p g l m) by reflexivity
   end.
 
 Ltac fold_L5 :=
   match goal with
-    |- context[model_UB ?RR (model_undef (Logic.eq) (interp_memory (interp_local_stack ?h (interp_global (interp_intrinsics ?ui ?p) ?g) ?l) ?m))] =>
-    replace (model_UB ?RR (model_undef (Logic.eq) (interp_memory (interp_local_stack h (interp_global (interp_intrinsics ui p) g) l) m))) with
-    (interp_to_L5 RR ui p g l m) by reflexivity
+    |- context[model_UB ?RR (model_undef (Logic.eq) (interp_memory (interp_local_stack ?h (interp_global (interp_intrinsics ?p) ?g) ?l) ?m))] =>
+    replace (model_UB ?RR (model_undef (Logic.eq) (interp_memory (interp_local_stack h (interp_global (interp_intrinsics p) g) l) m))) with
+    (interp_to_L5 RR p g l m) by reflexivity
   end.
